src/lib/state/DY.Lib.State.Map.fst
@@ -34,8 +34,8 @@ noeq type map_predicate {|crypto_invariants|} (key_t:eqtype) (value_t:Type0) {|m
   pred_knowable: tr:trace -> prin:principal -> sess_id:state_id -> key:key_t -> value:value_t -> Lemma
     (requires pred tr prin sess_id key value)
     (ensures
-      is_well_formed_prefix mt.ps_key_t (is_knowable_by (principal_tagged_state_label prin sess_id (tag #key_t #value_t)) tr) key /\
-      is_well_formed_prefix mt.ps_value_t (is_knowable_by (principal_tagged_state_label prin sess_id (tag #key_t #value_t)) tr) value
+      is_well_formed_prefix mt.ps_key_t (is_knowable_by (principal_tag_state_label prin (tag #key_t #value_t) sess_id) tr) key /\
+      is_well_formed_prefix mt.ps_value_t (is_knowable_by (principal_tag_state_label prin (tag #key_t #value_t) sess_id) tr) value
     )
   ;
 }
@@ -108,8 +108,8 @@ let map_session_invariant #cinvs #key_t #value_t #mt mpred = {
     FStar.Classical.forall_intro_2 (FStar.Classical.move_requires_2 (mpred.pred_later tr1 tr2 prin sess_id))
   );
   pred_knowable = (fun tr prin sess_id content ->
-    let pre1 = (is_knowable_by (principal_tagged_state_label prin sess_id (tag #key_t #value_t)) tr) in
-    let pre2 = (is_knowable_by (principal_typed_state_content_label prin sess_id (tag #key_t #value_t) content) tr) in
+    let pre1 = (is_knowable_by (principal_tag_state_label prin (tag #key_t #value_t) sess_id) tr) in
+    let pre2 = (is_knowable_by (principal_typed_state_content_label prin (tag #key_t #value_t) sess_id content) tr) in
     map_invariant_eq mpred tr prin sess_id content;
     for_allP_eq (is_well_formed_prefix (ps_map_elem key_t value_t) pre2) content.key_values;
     introduce forall x. map_elem_invariant mpred tr prin sess_id x ==> is_well_formed_prefix (ps_map_elem key_t value_t) pre2 x
